Hacking on ext_simplifier

uexp/src/uexp/core.lean
@@ -1,69 +1,84 @@
-inductive uexp (v : Type)
+inductive uexp : Type
 | zero : uexp
 | one : uexp
-| plus {} : uexp → uexp → uexp
-| mul {} : uexp → uexp → uexp
+| plus : uexp → uexp → uexp
+| mul : uexp → uexp → uexp
 | squash : uexp → uexp
 | not : uexp → uexp
-| var {} : v → uexp
+| var {} : string → uexp
 -- I don't fully understand the "typing" of sigma
-| sigma : (v → uexp) → uexp
+-- | sigma : (v → uexp) → uexp
 | equals : uexp → uexp → uexp
 | project : uexp → string → uexp
-| rel {} : string → v → uexp
+| rel : string → string → uexp
 | le : uexp → uexp → uexp
-| int {} : int → uexp
+| int : int → uexp
 
-instance uexp.has_zero (v : Type) : has_zero (uexp v) :=
-⟨ @uexp.zero v ⟩
+instance uexp.has_zero : has_zero uexp :=
+⟨ uexp.zero ⟩
 
-instance uexp.has_one (v : Type) : has_one (uexp v) :=
-⟨ @uexp.one v ⟩
+instance uexp.has_one : has_one uexp:=
+⟨ uexp.one ⟩
 
-instance uexp.has_add (v : Type) : has_add (uexp v) :=
+instance uexp.has_add : has_add uexp :=
 ⟨ uexp.plus ⟩
 
-instance uexp.has_mul (v : Type) : has_mul (uexp v) :=
+instance uexp.has_mul : has_mul uexp :=
 ⟨ uexp.mul ⟩
 
-instance uexp.var_coe (v : Type) : has_coe v (uexp v) :=
+instance uexp.var_coe : has_coe string uexp :=
 ⟨ uexp.var ⟩
 
 infix `=>`:61 := uexp.project
 infix `~=`:60 := uexp.equals
 
-inductive uexp.eq {v : Type} : uexp v → uexp v → Prop
-| refl : forall u1, uexp.eq u1 u1
--- rule 19
-| sigma_hoist :
-    forall E (f : v → uexp v),
-        uexp.eq (E * (@uexp.sigma v f)) (uexp.sigma (fun t', E * (f t')))
--- rule 16
-| add_comm : forall (E1 E2 : uexp v),
-  uexp.eq (E1 + E2) (E2 + E1)
-| add_func : forall (E1 E2 E3: uexp v),
-  uexp.eq E2 E3 → uexp.eq (E1 + E2)
-   (E1 + E3)
-| mul_assoc : forall (E1 E2 E3 : uexp v),
-  uexp.eq (E1 * (E2 * E3)) (E1 * E2 * E3)
-| mul_comm : forall (E1 E2 : uexp v),
-  uexp.eq (E1 * E2) (E2 * E1)
-| mul_distr : forall (E1 E2 E3: uexp v),
-  uexp.eq ((E1 + E2) * E3) (E1 * E3 + E2 * E3)
-| sigma_inj :
-    forall (f g : v → uexp v),
-        (forall (x : v), uexp.eq (f x) (g x)) →
-        uexp.eq (uexp.sigma f) (uexp.sigma g)
-| trans : forall (e1 e2 e3 : uexp v),
-    uexp.eq e1 e2 →
-    uexp.eq e2 e3 →
-    uexp.eq e1 e3
+inductive uexp.eq : uexp → uexp → Prop.
+
+-- | refl : forall u1, uexp.eq u1 u1
+-- -- -- rule 19
+-- -- | sigma_hoist :
+-- --     forall E (f : string → uexp),
+-- --         uexp.eq (E * (@uexp.sigma v f)) (uexp.sigma (fun t', E * (f t')))
+-- -- rule 16
+-- | add_comm : forall (E1 E2 : uexp),
+--   uexp.eq (uexp.plus E1 E2) (uexp.plus E2 E1)
+-- | add_func : forall (E1 E2 E3: uexp),
+--   uexp.eq E2 E3 → uexp.eq (E1 + E2)
+--    (E1 + E3)
+-- | mul_assoc : forall (E1 E2 E3 : uexp),
+--   uexp.eq (E1 * (E2 * E3)) (E1 * E2 * E3)
+-- | mul_comm : forall (E1 E2 : uexp),
+--   uexp.eq (E1 * E2) (E2 * E1)
+-- | mul_distr : forall (E1 E2 E3: uexp),
+--   uexp.eq ((E1 + E2) * E3) (E1 * E3 + E2 * E3)
+-- -- | sigma_inj :
+-- --     forall (f g : string → uexp),
+-- --         (forall (x : string), uexp.eq (f x) (g x)) →
+-- --         uexp.eq (uexp.sigma f) (uexp.sigma g)
+-- | trans : forall (e1 e2 e3 : uexp),
+--     uexp.eq e1 e2 →
+--     uexp.eq e2 e3 →
+--     uexp.eq e1 e3
 
 -- We need to add these to mark the relation as an equivalence relation for
 -- the simplifier.
-attribute [refl] uexp.eq.refl
-attribute [trans] uexp.eq.trans
+
 
 infix `≃`:50 := uexp.eq
+
+@[refl] lemma uexp_eq_refl :
+  forall (e1 : uexp), e1 ≃ e1 :=
+begin
+  admit
+end
+
+@[trans] lemma uexp_eq_trans :
+  forall (e1 e2 e3 : uexp),
+    e1 ≃ e2 →
+    e2 ≃ e3 →
+    e1 ≃ e3 :=
+begin
+  admit
+end
 
 open uexp
